FunMaps.v
@@ -15,12 +15,12 @@ Definition SetMap_AbsR {A B}
            (or : FunRel M.key A) (nr : M.t B)
            (AbsR : A -> B -> Prop) : Prop :=
   forall addr,
-    (forall data,
-       Lookup addr data or
-         -> (exists cdata, M.find addr nr = Some cdata /\ AbsR data cdata)) /\
-    (forall cdata,
-       M.find addr nr = Some cdata
-         -> (exists data, Lookup addr data or /\ AbsR data cdata)).
+    (forall blk,
+       Lookup addr blk or
+         -> (exists cblk, M.find addr nr = Some cblk /\ AbsR blk cblk)) /\
+    (forall cblk,
+       M.find addr nr = Some cblk
+         -> (exists blk, Lookup addr blk or /\ AbsR blk cblk)).
 
 Lemma Empty_SetMap_AbsR : forall A B R,
   SetMap_AbsR (Empty M.key A) (M.empty B) R.
@@ -41,8 +41,8 @@ Ltac reduction :=
     destruct (H1 A) as [HA HB]; clear H1;
     let HC := fresh "HC" in
     let HD := fresh "HD" in
-    destruct (HA _ H2) as [cdata [HC HD]]; clear HA HB H2;
-    exists cdata
+    destruct (HA _ H2) as [cblk [HC HD]]; clear HA HB H2;
+    exists cblk
   | [ H1 : SetMap_AbsR _ _ _,
       H2 : M.find ?A ?K = Some ?D |- _ ] =>
     let HA := fresh "HA" in
@@ -50,33 +50,53 @@ Ltac reduction :=
     destruct (H1 A) as [HA HB]; clear H1;
     let HC := fresh "HC" in
     let HD := fresh "HD" in
-    destruct (HB _ H2) as [data [HC HD]]; clear HA HB H2;
-    exists data
+    destruct (HB _ H2) as [blk [HC HD]]; clear HA HB H2;
+    exists blk
   end.
 
 Section FunMaps_AbsR.
 
 Variables A B : Type.
-Variable R    : A -> B -> Prop.
-Variable or   : FunRel M.key A.
-Variable nr   : M.t B.
-Variable H    : SetMap_AbsR or nr R.
+Variable R  : A -> B -> Prop.
+Variable or : FunRel M.key A.
+Variable nr : M.t B.
+Variable H  : SetMap_AbsR or nr R.
 
 Hypothesis Oeq_eq : forall a b, O.eq a b -> a = b.
 
 Lemma Find_find_if P P' a b b' :
   (forall i a b, R a b -> P i a <-> is_true (P' i b))
+    -> (forall a b c, R a b -> R a c -> b = c)
+    -> (forall (a b : M.key) (x y : B),
+          is_true (P' a x) -> ~ M.E.eq a b -> P' b y = false)
     -> R b b'
-    -> Find P a b or <-> find_if P' nr = Some (a, b').
+    -> Find P a b or
+    -> find_if P' nr = Some (a, b').
 Proof.
-  split; intros.
-    destruct H2.
-    eapply H0 in H3; eauto.
-    destruct (H a); clear H H5.
-    destruct (H4 _ H2); clear H2 H4.
-    destruct H; clear H.
-    unfold find_if.
-Abort.
+  intros.
+  destruct H4.
+  eapply H0 in H5; eauto; clear H0.
+  destruct (H a) as [H0 _]; clear H.
+  destruct (H0 _ H4) as [b'' [H H6]]; clear H4 H0.
+  unfold find_if.
+  rewrite F.elements_o in H.
+  rewrite M.fold_1.
+  induction (M.elements nr).
+    discriminate.
+  rewrite fold_Some_cons; auto.
+  destruct a0; simpl in *.
+  unfold F.eqb in H.
+  destruct (F.eq_dec a k).
+    pose proof (H1 _ _ _ H3 H6); subst.
+    clear H1 H2 H3 H6 IHl.
+    inversion H; clear H.
+    unfold M.E.eq in e.
+    apply Oeq_eq in e; subst.
+    rewrite H5.
+    reflexivity.
+  rewrite (IHl H), (H2 _ _ _ _ H5 n).
+  reflexivity.
+Qed.
 
 Lemma Update_SetMap_AbsR : forall k v v',
   R v v' -> SetMap_AbsR (Update k v or) (M.add k v' nr) R.
@@ -133,14 +153,14 @@ Proof.
   split; intros.
     teardown; subst.
     destruct (H addr); clear H H3.
-    destruct (H1 _ H2) as [cdata [? ?]]; clear H1 H2.
+    destruct (H1 _ H2) as [cblk [? ?]]; clear H1 H2.
     apply F.find_mapsto_iff in H.
-    exists (f' addr cdata).
+    exists (f' addr cblk).
     split.
       rewrite F.mapi_o, <- F.map_o.
         apply F.find_mapsto_iff.
         apply F.map_mapsto_iff.
-        exists cdata; tauto.
+        exists cblk; tauto.
       intros.
       apply Oeq_eq in H1.
       subst; reflexivity.
@@ -151,8 +171,8 @@ Proof.
     destruct H1; destruct H1; subst.
     apply F.find_mapsto_iff in H2.
     destruct (H addr); clear H H1.
-    destruct (H3 _ H2) as [data [? ?]]; clear H2 H3.
-    exists (f (addr, data)).
+    destruct (H3 _ H2) as [blk [? ?]]; clear H2 H3.
+    exists (f (addr, blk)).
     split.
       apply Lookup_Map; trivial.
     apply H0; trivial.
